---
layout: post
title: Change Of Basis
---

Here you go - Change Of Basis





Displayed equations
-------------------


$$
f(x) = 5x^{10}-9x^9 + 77x^8 + 12x^7 + 4x^6 - 8x^5 + 7x^4 + x^3 -2x^2 + 3x + 11.
$$

![_config.yml]({{ site.baseurl }}/images/changeOfBasis.jpg)

$$
\begin{aligned}
  (x-y)^2
  &= (x-y)(x-y) \\
  &= x^2 -yx - xy + y^2 \\
  &= x^2 -2xy +y^2.
\end{aligned}
$$

$$
\begin{aligned}
  3x-y&=0 & 2a+b &= 4 \\
  x+y &=1 & a-3b &=10
\end{aligned}
$$

$$
f(x) = \frac{x}{x-1} \text{ for $x\not=1$}.
$$


Relations and operations
------------------------

-   Equality-like: $x=2$, $x \not= 3$, $x \cong y$, $x \propto y$, $y\sim z$, $N
    \approx M$, $y \asymp z$, $P \equiv Q$.

-   Order: $x < y$, $y \le z$, $z \ge 0$, $x \preceq y$, $y\succ z$, $A
    \subseteq B$, $B \supset Z$.

Illustrating array:

$$
A\ =\ \left( \begin{array}{c|ccc}
& 1 & 2 & 3 \\ \hline
1&a_{11}&a_{12}&a_{13} \\
2&a_{21}&a_{22}&a_{23} \\
3&a_{31}&a_{32}&a_{33}
\end{array} \right)
$$
